Updated examples.

tests/Add.bpl
@@ -9,8 +9,7 @@ type State;
 
 var M: MType;
 var C: CType;
-var R: CType; 
-var N: CType;
+var R: CType;
 var C#init: CType;
 var St: [Actor]State;
 
@@ -65,8 +64,11 @@ procedure Net#anon$1#entry#2()
   assert {:msg "  Channel invariant might not hold on action entry (generated #6)"} 0 <= R[Net#c];
   assert {:msg "  Channel invariant might not hold on action entry (generated #7)"} 0 <= C[Net#c];
   assert {:msg "  Channel invariant might not hold on action entry (generated #8)"} R[Net#c] == 0;
-  assert {:msg "  12.3: Channel invariant might not hold on action entry"} R[Net#a] == (R[Net#c] + C[Net#c]);
-  assert {:msg "  13.3: Channel invariant might not hold on action entry"} R[Net#b] == (R[Net#c] + C[Net#c]);
+  assert {:msg "  Channel invariant might not hold on action entry (generated #9)"} R[Net#a] == (R[Net#c] + C[Net#c]);
+  assert {:msg "  Channel invariant might not hold on action entry (generated #10)"} R[Net#b] == (R[Net#c] + C[Net#c]);
+  assert {:msg "  Channel invariant might not hold on action entry (generated #11)"} (forall idx$: int :: 
+    (0 <= idx$) && (idx$ < (R[Net#c] + C[Net#c])) ==> (M[Net#c][idx$] == (M[Net#a][idx$] + M[Net#b][idx$]))
+  );
 }
 procedure Net#anon$1#Add#anon$0#3()
   modifies C, R, M, St;
@@ -88,6 +90,9 @@ procedure Net#anon$1#Add#anon$0#3()
   assume R[Net#c] == 0;
   assume R[Net#a] == (R[Net#c] + C[Net#c]);
   assume R[Net#b] == (R[Net#c] + C[Net#c]);
+  assume (forall idx$: int :: 
+    (0 <= idx$) && (idx$ < (R[Net#c] + C[Net#c])) ==> (M[Net#c][idx$] == (M[Net#a][idx$] + M[Net#b][idx$]))
+  );
   assume true;
   assume (1 <= C[Net#a]) && (1 <= C[Net#b]);
   in1#i := M[Net#a][R[Net#a]];
@@ -98,17 +103,20 @@ procedure Net#anon$1#Add#anon$0#3()
   C[Net#b] := C[Net#b] - 1;
   M[Net#c][R[Net#c] + C[Net#c]] := in1#i + in2#j;
   C[Net#c] := C[Net#c] + 1;
-  assert {:msg "  Sub-actor action at 3.3 might not preserve the channel invariant (generated #9)"} 0 <= R[Net#a];
-  assert {:msg "  Sub-actor action at 3.3 might not preserve the channel invariant (generated #10)"} 0 <= C[Net#a];
-  assert {:msg "  Sub-actor action at 3.3 might not preserve the channel invariant (generated #11)"} (R[Net#a] + C[Net#a]) == C#init[Net#a];
-  assert {:msg "  Sub-actor action at 3.3 might not preserve the channel invariant (generated #12)"} 0 <= R[Net#b];
-  assert {:msg "  Sub-actor action at 3.3 might not preserve the channel invariant (generated #13)"} 0 <= C[Net#b];
-  assert {:msg "  Sub-actor action at 3.3 might not preserve the channel invariant (generated #14)"} (R[Net#b] + C[Net#b]) == C#init[Net#b];
-  assert {:msg "  Sub-actor action at 3.3 might not preserve the channel invariant (generated #15)"} 0 <= R[Net#c];
-  assert {:msg "  Sub-actor action at 3.3 might not preserve the channel invariant (generated #16)"} 0 <= C[Net#c];
-  assert {:msg "  Sub-actor action at 3.3 might not preserve the channel invariant (generated #17)"} R[Net#c] == 0;
-  assert {:msg "  12.3: Sub-actor action at 3.3 might not preserve the channel invariant"} R[Net#a] == (R[Net#c] + C[Net#c]);
-  assert {:msg "  13.3: Sub-actor action at 3.3 might not preserve the channel invariant"} R[Net#b] == (R[Net#c] + C[Net#c]);
+  assert {:msg "  Sub-actor action at 3.3 might not preserve the channel invariant (generated #12)"} 0 <= R[Net#a];
+  assert {:msg "  Sub-actor action at 3.3 might not preserve the channel invariant (generated #13)"} 0 <= C[Net#a];
+  assert {:msg "  Sub-actor action at 3.3 might not preserve the channel invariant (generated #14)"} (R[Net#a] + C[Net#a]) == C#init[Net#a];
+  assert {:msg "  Sub-actor action at 3.3 might not preserve the channel invariant (generated #15)"} 0 <= R[Net#b];
+  assert {:msg "  Sub-actor action at 3.3 might not preserve the channel invariant (generated #16)"} 0 <= C[Net#b];
+  assert {:msg "  Sub-actor action at 3.3 might not preserve the channel invariant (generated #17)"} (R[Net#b] + C[Net#b]) == C#init[Net#b];
+  assert {:msg "  Sub-actor action at 3.3 might not preserve the channel invariant (generated #18)"} 0 <= R[Net#c];
+  assert {:msg "  Sub-actor action at 3.3 might not preserve the channel invariant (generated #19)"} 0 <= C[Net#c];
+  assert {:msg "  Sub-actor action at 3.3 might not preserve the channel invariant (generated #20)"} R[Net#c] == 0;
+  assert {:msg "  Sub-actor action at 3.3 might not preserve the channel invariant (generated #21)"} R[Net#a] == (R[Net#c] + C[Net#c]);
+  assert {:msg "  Sub-actor action at 3.3 might not preserve the channel invariant (generated #22)"} R[Net#b] == (R[Net#c] + C[Net#c]);
+  assert {:msg "  Sub-actor action at 3.3 might not preserve the channel invariant (generated #23)"} (forall idx$: int :: 
+    (0 <= idx$) && (idx$ < (R[Net#c] + C[Net#c])) ==> (M[Net#c][idx$] == (M[Net#a][idx$] + M[Net#b][idx$]))
+  );
 }
 procedure Net#anon$1#exit#4()
   modifies C, R, M, St;
@@ -128,6 +136,9 @@ procedure Net#anon$1#exit#4()
   assume R[Net#c] == 0;
   assume R[Net#a] == (R[Net#c] + C[Net#c]);
   assume R[Net#b] == (R[Net#c] + C[Net#c]);
+  assume (forall idx$: int :: 
+    (0 <= idx$) && (idx$ < (R[Net#c] + C[Net#c])) ==> (M[Net#c][idx$] == (M[Net#a][idx$] + M[Net#b][idx$]))
+  );
   assume !((1 <= C[Net#a]) && (1 <= C[Net#b]));
   assert {:msg "  8.3: The network might leave unread tokens on channel a"} C[Net#a] == 0;
   assert {:msg "  8.3: The network might leave unread tokens on channel b"} C[Net#b] == 0;
